feat: tuple_spec

src/Set Theory: An Open Introduction/9 Steps towards Z.lean
@@ -44,9 +44,6 @@ def subset (A B : Set) :=
 
 instance : has_subset Set := ⟨subset⟩
 
--- Axiom (Extensionality). For any sets A and B: ∀ x (x ∈ A ↔ x ∈ B) → A = B
-@[ext] axiom extensionality (A B : Set) (h : ∀ x, x ∈ A ↔ x ∈ B) : A = B
-
 -- Theorem 8.1 (Russell’s Paradox). There is no set R = {x : x ∉ x}
 theorem russell's_paradox : ¬ ∃ R : Set, ∀ x, x ∈ R ↔ x ∉ x :=
 begin
@@ -58,6 +55,17 @@ end
 -- no (ZFC) axioms
 #print axioms russell's_paradox
 
+-- Axiom (Extensionality). For any sets A and B: ∀ x (x ∈ A ↔ x ∈ B) → A = B
+@[ext] axiom extensionality (A B : Set) (h : ∀ x, x ∈ A ↔ x ∈ B) : A = B
+
+#check @set.ext_iff
+
+lemma ext_iff {A B : Set} : A = B ↔ ∀ x, x ∈ A ↔ x ∈ B :=
+begin
+  have := extensionality A B,
+  tidy
+end
+
 #print notation ↔
 #print notation ∧
 
@@ -68,6 +76,10 @@ end
 -- any A, the set {x ∈ A : φ(x)} exists.
 axiom separation (φ : Set → Prop) (A : Set) : Set
 axiom separation_spec (φ : Set → Prop) (A : Set) : ∀ x, x ∈ separation φ A ↔ x ∈ A ∧ φ x
+
+#check @has_sep
+
+instance : has_sep Set Set := ⟨separation⟩
 
 -- Theorem 9.1. There is no universal set, i.e., {x : x = x} does not exist.
 theorem not_exists_universal_set : ¬ ∃ V : Set, ∀ x, x ∈ V :=
@@ -128,7 +140,7 @@ end
 -- Axiom (Union). For any set A, the set ⋃︁ A = {x : (∃ b ∈ A) x ∈ b} exists.
 -- ∀ A ∃ U ∀ x (x ∈ U ↔ (∃ b ∈ A) x ∈ b)
 axiom union (A : Set) : Set
-axiom union_spec (A : Set) : ∀ x, x ∈ union A ↔ ∃ b ∈ A, x ∈ b
+axiom union_spec (A : Set) : ∀ x, x ∈ union A ↔ ∃ b, b ∈ A ∧ x ∈ b
 
 #print notation ↔
 #print notation ∨
@@ -155,7 +167,7 @@ axiom infinity_spec_succ : ∀ x ∈ infinity, ∃ s ∈ infinity, ∀ z, z ∈ 
 
 instance : has_emptyc Set := ⟨separation (λ x, false) infinity⟩
 
-lemma empty_spec : ∀ x : Set, x ∉ (∅ : Set) :=
+lemma empty_spec : ∀ x, x ∉ (∅ : Set) :=
 begin
   intros x hx,
   change x ∈ separation _ _ at hx,
@@ -174,4 +186,226 @@ begin
   have h₁ := empty_spec x,
   have h₂ := ho₂ x,
   simp [h₁, h₂]
+end
+
+--def closed (f : Set → Set) (X : Set) := ∀ x, x ∈ X → f x ∈ X
+
+-- Proposition 9.5. For any sets a and b, the following sets exist:
+-- 1. {a}
+-- 2. a ∪ b
+-- 3. ⟨a,b⟩
+instance : has_singleton Set Set := ⟨λ a, pair a a⟩
+
+lemma singleton_spec (a : Set) : ∀ x ∈ ({a} : Set), x = a :=
+begin
+  intros x hx,
+  change x ∈ pair a a at hx,
+  have h := pair_spec a a,
+  change x ∈ {a} at hx,
+  change ∀ x, x ∈ ({a} : Set) ↔ _ at h,
+  specialize h x,
+  simpa [hx] using h
+end
+
+#check @has_union
+#check @has_union.union
+#print notation ∪
+
+instance : has_union Set := ⟨λ a b, union (pair a b)⟩
+
+lemma union_spec' (a b : Set) : ∀ x, x ∈ a ∪ b ↔ x ∈ a ∨ x ∈ b :=
+begin
+  intro x,
+  change x ∈ union (pair a b) ↔ _,
+  have h := union_spec (pair a b),
+  specialize h x,
+  rw h,
+  clear h,
+  have h := pair_spec a b,
+  split,
+  { rintro ⟨c, hc₁, hc₂⟩,
+    specialize h c,
+    simp [hc₁] at h,
+    cases h,
+    { rw ←h,
+      left,
+      assumption },
+    { rw ←h,
+      right,
+      assumption } },
+  { intro hx,
+    cases hx,
+    { use a,
+      specialize h a,
+      simp at h,
+      simp [h, hx] },
+    { use b,
+      specialize h b,
+      simp at h,
+      simp [h, hx] } }
+end
+
+#check @has_insert
+
+instance : has_insert Set Set := ⟨λ a b, {a} ∪ b⟩
+
+instance : is_lawful_singleton Set Set :=
+⟨begin
+  change ∀ x, {x} ∪ ∅ = {x},
+  intro x,
+  ext y,
+  simp [union_spec', empty_spec]
+end⟩
+
+example {α : Type} (a b : α) (h : a ∈ ({b} : set α)) : a = b :=
+set.mem_singleton_iff.mp h
+
+#check @set.mem_singleton_iff
+
+lemma mem_singleton_iff {a b : Set} : a ∈ ({b} : Set) ↔ a = b :=
+begin
+  change a ∈ pair b b ↔ _,
+  have := pair_spec b b a,
+  simp [this]
+end
+
+variables {a b c : Set}
+
+#check ({a, b, c} : Set)
+
+variables {a₁ a₂ b₁ b₂ : Set}
+
+#check extensionality
+#check set.ext_iff
+
+lemma pair_spec' (a b : Set) : pair a b = {a, b} :=
+begin
+  ext x,
+  have := pair_spec a b x,
+  rw this,
+  clear this,
+  change _ ↔ x ∈ {a} ∪ {b},
+  have := union_spec' {a} {b} x,
+  rw [this, mem_singleton_iff, mem_singleton_iff]
+end
+
+lemma eq_of_eq_singleton (h : {b₁, b₂} = ({a} : Set)) : b₁ = b₂ := 
+begin
+  have h₁ : b₁ = a,
+  { have := ext_iff.mp h b₁,
+    rw [←pair_spec', mem_singleton_iff, pair_spec b₁ b₂ b₁] at this,
+    simpa using this },
+  have h₂ : b₂ = a,
+  { have := ext_iff.mp h b₂,
+    rw [←pair_spec', mem_singleton_iff, pair_spec b₁ b₂ b₂] at this,
+    simpa using this },
+  rw [h₁, h₂]
+end
+
+def tuple (a b : Set) : Set := pair (pair a a) (pair a b)
+
+#check singleton_spec
+
+example {α : Type} (a b : α) (h : ({a} : set α) = {b}) : a = b :=
+by simpa only [set.singleton_eq_singleton_iff] using h
+
+lemma singleton_eq_singleton_iff {a b : Set} : ({a} : Set) = {b} ↔ a = b :=
+begin
+  split,
+  { intro h,
+    have : a ∈ {b}, by rw [←h, mem_singleton_iff],
+    rwa mem_singleton_iff at this },
+  { intro h,
+    rw h }
+end
+
+lemma fst_eq_fst_of_tuple_eq_tuple (h : tuple a₁ b₁ = tuple a₂ b₂) : a₁ = a₂ :=
+begin
+  have h' : pair a₂ a₂ ∈ tuple a₁ b₁,
+  { rw h,
+    have := pair_spec (pair a₂ a₂) (pair a₂ b₂) (pair a₂ a₂),
+    simpa using this },
+  unfold tuple at h',
+  have := pair_spec (pair a₁ a₁) (pair a₁ b₁) (pair a₂ a₂),
+  simp [h'] at this,
+  clear h h',
+  cases this,
+  { change {a₂} = {a₁} at this,
+    rw ←singleton_eq_singleton_iff,
+    symmetry,
+    assumption },
+  { suffices h : a₁ = b₁,
+    { subst h,
+      change {a₂} = {a₁} at this,
+      rw ←singleton_eq_singleton_iff,
+      symmetry,
+      assumption },
+    change {a₂} = _ at this,
+    have h := pair_spec' a₁ b₁,
+    rw h at this,
+    clear h,
+    have := eq_of_eq_singleton (this).symm,
+    assumption }
+end
+
+example {α : Type} (a b : α) : a = b ↔ b = a :=
+eq_comm
+
+lemma pair_eq_singleton (a : Set) : pair a a = {a} :=
+begin
+  ext,
+  have := pair_spec a a x,
+  simp [this, mem_singleton_iff]
+end
+
+lemma mem_pair_left (a b : Set) : a ∈ pair a b :=
+begin
+  have := pair_spec a b a,
+  simpa using this
+end
+
+lemma mem_pair_right (a b : Set) : b ∈ pair a b :=
+begin
+  have := pair_spec a b b,
+  simpa using this
+end
+
+lemma snd_eq_snd_of_tuple_eq_tuple (h : tuple a₁ b₁ = tuple a₂ b₂) : b₁ = b₂ :=
+begin
+  obtain rfl := fst_eq_fst_of_tuple_eq_tuple h,
+  rename a₁ a,
+  have h' : pair a b₂ ∈ tuple a b₁,
+  { rw h,
+    have := pair_spec (pair a a) (pair a b₂) (pair a b₂),
+    simpa using this },
+  unfold tuple at h',
+  have := pair_spec (pair a a) (pair a b₁) (pair a b₂),
+  simp [h'] at this,
+  cases this,
+  { have : a = b₂,
+    { change _ = {a} at this,
+      rw pair_spec' at this,
+      simp [eq_of_eq_singleton this] },
+    subst this,
+    clear this,
+    unfold tuple at h,
+    rw [pair_eq_singleton, pair_eq_singleton, pair_spec', pair_spec'] at h,
+    have h := eq_of_eq_singleton h,
+    have h := eq_of_eq_singleton h.symm,
+    rw h },
+  { clear h h',
+    have h₁ := pair_spec a b₁ b₂,
+    rw ←this at h₁,
+    simp [mem_pair_right] at h₁,
+    have h₂ := pair_spec a b₂ b₁,
+    rw this at h₂,
+    simp [mem_pair_right] at h₂,
+    cases h₁; cases h₂; tidy }
+end
+
+lemma tuple_spec : tuple a₁ b₁ = tuple a₂ b₂ ↔ a₁ = a₂ ∧ b₁ = b₂ :=
+begin
+  split; intro h,
+  { simp [fst_eq_fst_of_tuple_eq_tuple h, snd_eq_snd_of_tuple_eq_tuple h] },
+  { simp [h] }
 end
